implemented Otway-Rees messages and serialization function

otway-rees/OYRS.Debug.fst
@@ -1,1 +1,44 @@
 module OYRS.Debug
+
+
+open SecrecyLabels
+open CryptoEffect
+open CryptoLib
+open GlobalRuntimeLib
+open LabeledCryptoAPI
+open LabeledRuntimeAPI
+open LabeledPKI
+open AttackerAPI
+open ORYS.Sessions
+open ORYS.Protocol
+
+
+val benign_attacker:
+  unit ->
+  LCrypto unit (pki nsl_preds)
+  (requires fun _ -> True)
+  (ensures fun _ _ _ -> True)
+
+#set-options "--z3rlimit 200 --max_fuel 4 --max_ifuel 2"
+let benign_attacker () =
+  ()
+
+let benign () : LCrypto unit (pki nsl_preds)
+  (requires (fun _ -> True)) (ensures (fun _ _ _ -> True))
+= print_string "start\n";
+  let t0 = get() in
+  let x = benign_attacker () in
+  print_trace ()
+
+let main =
+  IO.print_string "======================\n";
+  IO.print_string "Otway-Rees            \n";
+  IO.print_string "======================\n";
+  let t0 = Seq.empty in
+  IO.print_string "Starting Benign Attacker:\n";
+  assume(valid_trace (pki nsl_preds) t0);
+  let r,t1 = (reify (benign ()) t0) in
+  (match r with
+  | Error s -> IO.print_string ("ERROR: "^s^"\n")
+  | Success _ -> IO.print_string "PROTOCOL RUN: Successful execution of Otway-Rees protocol.\n");
+  IO.print_string "Finished Benign Attacker:\n"
