otway-rees/OYRS.Messages.fst
@@ -1,1 +1,31 @@
 module OYRS.Messages
+
+
+module LC = LabeledCryptoAPI
+
+
+let valid_message i (m:message i) =
+  match m with
+  | Msg1 c a b ev_a -> LC.is_msg oyrs_global_usage i c public
+  | Msg2 c a b ev_a ev_b -> LC.is_msg oyrs_global_usage i c public
+  | Msg3 c ev_a ev_b -> LC.is_msg oyrs_global_usage i c public
+  | Msg4 c ev_a -> LC.is_msg oyrs_global_usage i c public
+
+let serialize_msg i m =
+  match m with
+  | Msg1 c a b ev_a ->
+    let tag = (LC.string_to_bytes #oyrs_global_usage #i "msg1") in
+    let a_bytes = (LC.string_to_bytes #oyrs_global_usage #i a) in
+    let b_bytes = (LC.string_to_bytes #oyrs_global_usage #i b) in
+    LC.concat #oyrs_global_usage #i #public tag (LC.concat #oyrs_global_usage #i #public c (LC.concat #oyrs_global_usage #i #public a_bytes (LC.concat #oyrs_global_usage #i #public b_bytes ev_a)))
+  | Msg2 c a b ev_a ev_b ->
+    let tag = (LC.string_to_bytes #oyrs_global_usage #i "msg2") in
+    let a_bytes = (LC.string_to_bytes #oyrs_global_usage #i a) in
+    let b_bytes = (LC.string_to_bytes #oyrs_global_usage #i b) in
+    LC.concat #oyrs_global_usage #i #public tag (LC.concat #oyrs_global_usage #i #public c (LC.concat #oyrs_global_usage #i #public a_bytes (LC.concat #oyrs_global_usage #i #public b_bytes (LC.concat #oyrs_global_usage #i #public ev_a ev_b))))
+  | Msg3 c ev_a ev_b ->
+    let tag = (LC.string_to_bytes #oyrs_global_usage #i "msg3") in
+    LC.concat #oyrs_global_usage #i #public tag (LC.concat #oyrs_global_usage #i #public c (LC.concat #oyrs_global_usage #i #public ev_a ev_b))
+  | Msg4 c ev_a ->
+    let tag = (LC.string_to_bytes #oyrs_global_usage #i "msg4") in
+    LC.concat #oyrs_global_usage #i #public tag (LC.concat #oyrs_global_usage #i #public c ev_a)
