otway-rees/OYRS.Messages.fsti
@@ -1,0 +1,48 @@
+module OYRS.Messages
+
+
+open SecrecyLabels
+open GlobalRuntimeLib
+open CryptoLib
+
+module LC = LabeledCryptoAPI
+
+
+/// Encrypted message parts
+noeq type encval =
+  | EncMsg1: n_a:bytes -> c:bytes -> a:string -> b:string -> encval
+  | EncMsg2: n_b:bytes -> c:bytes -> a:string -> b:string -> encval
+  | EncMsg3_I: n_a:bytes -> k_ab:bytes -> encval
+  | EncMsg3_R: n_b:bytes -> k_ab:bytes -> encval
+
+let oyrs_key_usages : LC.key_usages = LC.default_key_usages
+
+let can_pke_encrypt (i:nat) s pk m = True
+let can_aead_encrypt i s k m ad = True
+let can_sign i s k m = True
+let can_mac i s k m = True
+
+let oyrs_usage_preds : LC.usage_preds = {
+  LC.can_pke_encrypt = can_pke_encrypt;
+  LC.can_aead_encrypt =  can_aead_encrypt;
+  LC.can_sign = can_sign;
+  LC.can_mac = can_mac
+}
+
+let oyrs_global_usage : LC.global_usage = {
+  LC.key_usages = oyrs_key_usages;
+  LC.usage_preds = oyrs_usage_preds;
+}
+
+let msg i l = LC.msg oyrs_global_usage i l
+
+noeq type message (i:nat) =
+  | Msg1: c:bytes -> a:string -> b:string -> ev_a:msg i public -> message i
+  | Msg2: c:bytes -> a:string -> b:string -> ev_a:msg i public -> ev_b:msg i public -> message i
+  | Msg3: c:bytes -> ev_a:msg i public -> ev_b:msg i public -> message i
+  | Msg4: c:bytes -> ev_a:msg i public -> message i
+
+val valid_message: i:nat -> m:(message i) -> Type0
+
+val serialize_msg: i:nat -> m:(message i){valid_message i m} -> msg i public
+val parse_msg: #i:nat -> msg i public -> result (message i)
