otway-rees/OYRS.Protocol.fsti
@@ -1,1 +1,49 @@
 module OYRS.Protocol
+
+
+open CryptoEffect
+open CryptoLib
+open GlobalRuntimeLib
+open ORYS.Messages
+open ORYS.Sessions
+open LabeledCryptoAPI
+open LabeledRuntimeAPI
+open LabeledPKI
+
+
+val initiator_send_msg_1:
+  initiator:principal ->
+  responder:principal ->
+  LCrypto (state_session_idx:nat * message_idx:nat) (pki oyrs_preds)
+  (requires fun t0 -> True)
+  (ensures fun t0 (si, msg_idx) t1 -> msg_idx < trace_len t1 /\ (trace_len t0 < trace_len t1))
+
+val responder_send_msg_2:
+  responder:principal ->
+  message_idx: nat ->
+  LCrypto (state_session_idx:nat * message_idx:nat) (pki orys_preds)
+  (requires fun t0 ->  message_idx < trace_len t0)
+  (ensures fun t0 (si, msg_idx) t1 -> msg_idx < trace_len t1 /\ (trace_len t0 < trace_len t1))
+
+val server_send_msg_3:
+  server:principal ->
+  message_idx: nat ->
+  LCrypto (state_session_idx:nat * message_idx:nat) (pki oyrs_preds)
+  (requires fun t0 ->  message_idx < trace_len t0)
+  (ensures fun t0 (si, msg_idx) t1 -> msg_idx < trace_len t1 /\ (trace_len t0 < trace_len t1))
+
+val responder_send_msg_4:
+  responder:principal ->
+  sess_idx_resp:nat ->
+  message_idx:nat ->
+  LCrypto (message_idx:nat) (pki oyrs_preds)
+  (requires fun t0 ->  msg_idx < trace_len t0)
+  (ensures fun t0 msg_idx t1 -> msg_idx < trace_len t1 /\ (trace_len t0 < trace_len t1))
+
+val initiator_recv_msg_4:
+  initiator:principal ->
+  sess_idx_init:nat ->
+  message_idx:nat ->
+  LCrypto unit (pki oyrs_preds)
+  (requires fun t0 -> message_idx < trace_len t0)
+  (ensures fun t0 _ t1 -> True)
